commit

Bidir.v
@@ -1,13 +1,12 @@
 Require Import Snoclist.
 Import SnoclistNotations.
 Require Import Types.
-
+Require Import Subst.
 Require Import LabeledLambda.
 
+Require Import Coq.Program.Equality.
+Require Import Coq.Sorting.Permutation.
 Require List.
-
-Definition type_eq : Type := type * type.
-Definition constraints : Type := list type_eq.
 
 Inductive is_bidir_syn : forall {a : nat}, context a -> sterm a -> type -> constraints -> Prop :=
 | bidir_abs {n} ty1 gamma (st : sterm (S n)) ty2 const :
@@ -22,7 +21,7 @@ with is_bidir_chk : forall {a : nat}, context a -> cterm a -> type -> constraint
 | bidir_app {n m} gamma delta (ct1 : cterm n) (st2 : sterm m) ty1 ty2 const1 const2 :
   is_bidir_chk gamma ct1 (TImp ty1 ty2) const1 ->
   is_bidir_syn delta st2 ty1 const2 ->
-  is_bidir_chk (gamma ++ delta) (CApp ct1 st2) ty2 (List.app const1 const2)
+  is_bidir_chk (gamma ++ delta) (CApp ct1 st2) ty2 (List.app const2 const1)
 | bidir_squ {n} gamma (st : sterm n) ty1 ty2 const :
   is_bidir_syn gamma st ty1 const ->
   is_bidir_chk gamma (CSqu st) ty2 (List.cons (ty1, ty2) const).
@@ -34,3 +33,134 @@ Inductive is_bidir : forall {a : nat}, context a -> lterm a -> type -> constrain
 | Cbidir {n} gamma (ct : cterm n) ty const :
   is_bidir_chk gamma ct ty const ->
   is_bidir gamma (LChk ct) ty const.
+
+Inductive sat_xi : s_rules -> constraints -> Prop :=
+| sat_nil sigma : sat_xi sigma List.nil
+| sat_cons sigma ty1 ty2 const :
+  sat_xi sigma const ->
+  subst_ty sigma ty1 = subst_ty sigma ty2 ->
+  sat_xi sigma (List.cons (ty1, ty2) const).
+
+Lemma app_sat_xi : forall (sigma : s_rules) (const1 const2 : constraints),
+  sat_xi sigma const1 -> sat_xi sigma const2 -> sat_xi sigma (const1 ++ const2)%list.
+Proof.
+intros sigma const1 const2 h1 h2.
+induction const1.
+- simpl. apply h2.
+- simpl.
+  dependent destruction h1.
+  apply sat_cons.
+  apply IHconst1.
+  apply h1.
+  apply H.
+Qed.
+
+Lemma perm_sat_xi : forall (sigma : s_rules) (const1 const2 : constraints),
+  Permutation const1 const2 -> sat_xi sigma const1 -> sat_xi sigma const2.
+Proof.
+intros sigma const1 const2 hp.
+induction hp.
+- intro hs. apply hs.
+- case x. intros ty1 ty2.
+  intro hs. dependent destruction hs.
+  apply sat_cons.
+  + apply IHhp. apply hs.
+  + apply H.
+- case x. intros ty1 ty2.
+  case y. intros ty1' ty2'.
+  intro hs.
+  dependent destruction hs.
+  dependent destruction hs.
+  apply sat_cons. apply sat_cons.
+  + apply hs.
+  + apply H0.
+  + apply H.
+- intro hl.
+  apply IHhp2.
+  apply IHhp1.
+  apply hl.
+Qed.
+
+Lemma extra_sat_xi : forall (sigma : s_rules) (x : type_eq) (const : constraints),
+  sat_xi sigma (x :: const)%list -> sat_xi sigma const.
+Proof. intros. dependent destruction H. apply H. Qed.
+
+Lemma appleft_sat_xi : forall (sigma : s_rules) (const1 const2 : constraints),
+  sat_xi sigma (List.app const1 const2) -> sat_xi sigma const1.
+Proof.
+induction const2.
+- rewrite List.app_nil_r. intro h. apply h.
+- intro h. apply IHconst2.
+  assert (Permutation (const1 ++ a :: const2)%list (a :: (const1 ++ const2))%list).
+  apply (Permutation_sym (Permutation_cons_app
+    (l := (const1 ++ const2)) const1 const2 a
+    (Permutation_refl (const1 ++ const2)))).
+  assert (sat_xi sigma (a :: const1 ++ const2)%list).
+  apply perm_sat_xi with (const1 := (const1 ++ a :: const2)%list).
+  apply H. apply h.
+  apply extra_sat_xi with (x := a).
+  apply H0.
+Qed.
+
+Lemma appright_sat_xi : forall (sigma : s_rules) (const1 const2 : constraints),
+  sat_xi sigma (List.app const1 const2) -> sat_xi sigma const2.
+Proof.
+induction const1.
+- simpl. intros const2 h. apply h.
+- intros const2 h. apply IHconst1.
+  simpl in h.
+  apply extra_sat_xi with (x := a).
+  apply h.
+Qed.
+
+Theorem bidir_typed_syn :
+  forall {n : nat} (gamma : context n) (st : sterm n) (ty : type) (const : constraints) (sigma : s_rules),
+  is_bidir_syn gamma st ty const ->
+  sat_xi sigma const ->
+  is_typed (subst_ctx sigma gamma) (strip_syn st) (subst_ty sigma ty)
+
+with bidir_typed_chk :
+  forall {n : nat} (gamma : context n) (ct : cterm n) (ty : type) (const : constraints) (sigma : s_rules),
+  is_bidir_chk gamma ct ty const ->
+  sat_xi sigma const ->
+  is_typed (subst_ctx sigma gamma) (strip_chk ct) (subst_ty sigma ty).
+
+Proof.
+- intros n gamma st ty const sigma hb hs.
+  induction hb.
+  + simpl.
+    rewrite dist_subst_ty.
+    apply typed_abs.
+    rewrite <- cons_subst_ctx.
+    apply IHhb. apply hs.
+  + simpl.
+    apply bidir_typed_chk
+    with (const := const).
+    apply H. apply hs.
+- intros n gamma ct ty const sigma hb hs.
+  induction hb.
+  + simpl.
+    rewrite single_subst_ctx.
+    apply (typed_var (subst_ty sigma ty)).
+  + simpl.
+    rewrite app_subst_ctx.
+    apply typed_app
+    with (ty1 := (subst_ty sigma ty1)).
+    * rewrite <- dist_subst_ty.
+      apply IHhb.
+      apply appright_sat_xi
+      with (const1 := const2).
+      apply hs.
+    * apply bidir_typed_syn
+      with (const := const2).
+      apply H.
+      apply appleft_sat_xi
+      with (const2 := const1).
+      apply hs.
+  + simpl.
+    dependent destruction hs.
+    rewrite <- H0.
+    apply bidir_typed_syn
+    with (const := const).
+    apply H. apply hs.
+Qed.
